Simplfied proofs.

theories/MACCCA.v
@@ -66,10 +66,10 @@ Context (dec: Word -> Word -> Word).
 Notation " 'word " := (Word) (in custom pack_type at level 2).
 Notation " 'word " := (Word) (at level 2): package_scope.
 
-Definition mac_key_location: Location := ('option 'word ; 0).
-Definition mac_set_location: Location := ('set ('word × 'word) ; 1).
-Definition enc_key_location: Location := ('option 'word ; 2).
-Definition cca_set_location: Location := ('set ('word × 'word) ; 3).
+Definition km_loc: Location := ('option 'word ; 0).
+Definition T_loc: Location := ('set ('word × 'word) ; 1).
+Definition ek_loc: Location := ('option 'word ; 2).
+Definition S_loc: Location := ('set ('word × 'word) ; 3).
 Definition gettag: nat := 4.
 Definition checktag: nat := 5.
 Definition eavesdrop: nat := 6.
@@ -79,27 +79,35 @@ Definition mkpair {Lt Lf E}
   (t: package Lt [interface] E) (f: package Lf [interface] E):
   loc_GamePair E := fun b => if b then {locpackage t} else {locpackage f}.
 
-Definition TAG_locs_tt := fset [:: mac_key_location].
-Definition TAG_locs_ff := fset [:: mac_key_location; mac_set_location].
+Definition TAG_locs_tt := fset [:: km_loc].
+Definition TAG_locs_ff := fset [:: km_loc; T_loc].
 
-Definition kgen {L I l} (_: ('option 'word ; l) \in L): code L I 'word :=
-  {code
-    k_init ← get ('option 'word ; l) ;;
-    match k_init with
-    | None =>
-        k <$ uniform Word_N ;;
-        #put ('option 'word ; l) := Some k ;;
-        ret k
-    | Some k =>
-        ret k
-    end
-  }.
+Definition kgen (l: Location): raw_code 'word :=
+  k_init ← get ('option 'word ; projT2 l) ;;
+  match k_init with
+  | None =>
+      k <$ uniform Word_N ;;
+      #put ('option 'word ; projT2 l) := Some k ;;
+      ret k
+  | Some k => ret k
+  end.
 
-Lemma TAG_locs_tt_key:
-  mac_key_location \in TAG_locs_tt.
+Lemma kgen_valid {L I} (l: nat):
+  ('option 'word ; l) \in L ->
+  ValidCode L I (kgen ('option 'word ; l)).
 Proof.
-  auto_in_fset.
+  move=> H.
+  apply: valid_getr => [// | [k|]].
+  1: by apply: valid_ret.
+  apply: valid_sampler => k.
+  apply: valid_putr => //.
+  by apply: valid_ret => //.
 Qed.
+
+Hint Extern 1 (ValidCode ?L ?I (kgen ?l)) =>
+  eapply kgen_valid ;
+  auto_in_fset
+  : typeclass_instances ssprove_valid_db.
 
 Definition TAG_pkg_tt:
   package TAG_locs_tt
@@ -109,20 +117,14 @@ Definition TAG_pkg_tt:
       #val #[checktag]: 'word × 'word → 'bool ] :=
   [package
     #def #[gettag] (m: 'word): 'word {
-      k ← kgen TAG_locs_tt_key ;;
+      k ← kgen km_loc ;;
       ret (mac k m)
     } ;
     #def #[checktag] ('(m, t): 'word × 'word): 'bool {
-      k ← kgen TAG_locs_tt_key ;;
-      ret (t == (mac k m))
+      k ← kgen km_loc ;;
+      ret (t == mac k m)
     }
   ].
-
-Lemma TAG_locs_ff_key:
-  mac_key_location \in TAG_locs_ff.
-Proof.
-  auto_in_fset.
-Qed.
 
 Definition TAG_pkg_ff:
   package TAG_locs_ff
@@ -132,34 +134,28 @@ Definition TAG_pkg_ff:
       #val #[checktag]: 'word × 'word → 'bool ] :=
   [package
     #def #[gettag] (m: 'word): 'word {
-      T ← get mac_set_location ;;
-      k ← kgen TAG_locs_ff_key ;;
+      T ← get T_loc ;;
+      k ← kgen km_loc ;;
       let t := mac k m in
-      #put mac_set_location := (setm T (m, t) tt) ;;
+      #put T_loc := setm T (m, t) tt ;;
       ret t
     } ;
     #def #[checktag] ('(m, t): 'word × 'word): 'bool {
-      T ← get mac_set_location ;;
+      T ← get T_loc ;;
       ret ((m, t) \in domm T)
     }
   ].
 
 Definition TAG := mkpair TAG_pkg_tt TAG_pkg_ff.
 
-Definition CPA_EVAL_locs := fset [:: enc_key_location].
-
-Lemma CPA_EVAL_locs_key:
-  enc_key_location \in CPA_EVAL_locs.
-Proof.
-  auto_in_fset.
-Qed.
+Definition CPA_EVAL_locs := fset [:: ek_loc].
 
 Definition CPA_EVAL_pkg_tt:
   package CPA_EVAL_locs [interface]
     [interface #val #[eavesdrop]: 'word × 'word → 'word ] :=
   [package
     #def #[eavesdrop] ('(ml, mr): 'word × 'word): 'word {
-      k ← kgen CPA_EVAL_locs_key ;;
+      k ← kgen ek_loc ;;
       ret (enc k ml)
     }
   ].
@@ -169,26 +165,14 @@ Definition CPA_EVAL_pkg_ff:
     [interface #val #[eavesdrop]: 'word × 'word → 'word ] :=
   [package
     #def #[eavesdrop] ('(ml, mr): 'word × 'word): 'word {
-      k ← kgen CPA_EVAL_locs_key ;;
+      k ← kgen ek_loc ;;
       ret (enc k mr)
     }
   ].
 
 Definition CPA_EVAL := mkpair CPA_EVAL_pkg_tt CPA_EVAL_pkg_ff.
 
-Definition CCA_EVAL_locs := fset [:: mac_key_location; enc_key_location; cca_set_location].
-
-Lemma CCA_EVAL_locs_mac_key:
-  mac_key_location \in CCA_EVAL_locs.
-Proof.
-  auto_in_fset.
-Qed.
-
-Lemma CCA_EVAL_locs_enc_key:
-  enc_key_location \in CCA_EVAL_locs.
-Proof.
-  auto_in_fset.
-Qed.
+Definition CCA_EVAL_locs := fset [:: km_loc; ek_loc; S_loc].
 
 Definition CCA_EVAL_pkg_tt:
   package CCA_EVAL_locs [interface]
@@ -197,20 +181,20 @@ Definition CCA_EVAL_pkg_tt:
       #val #[decrypt]: 'word × 'word → 'option 'word ] :=
   [package
     #def #[eavesdrop] ('(ml, mr): 'word × 'word): 'word × 'word {
-      S ← get cca_set_location ;;
-      ke ← kgen CCA_EVAL_locs_enc_key ;;
-      km ← kgen CCA_EVAL_locs_mac_key ;;
+      S ← get S_loc ;;
+      ke ← kgen ek_loc ;;
+      km ← kgen km_loc ;;
       let c := enc ke ml in
       let t := mac km c in
-      #put cca_set_location := (setm S (c, t) tt) ;;
+      #put S_loc := setm S (c, t) tt ;;
       ret (c, t)
     } ;
     #def #[decrypt] ('(c, t): 'word × 'word): 'option 'word {
-      S ← get cca_set_location ;;
+      S ← get S_loc ;;
       if ((c, t) \in domm S) then ret None else
-      km ← kgen CCA_EVAL_locs_mac_key ;;
+      km ← kgen km_loc ;;
       if (t != mac km c) then ret None else
-      ke ← kgen CCA_EVAL_locs_enc_key ;;
+      ke ← kgen ek_loc ;;
       ret (Some (dec ke c))
     }
   ].
@@ -222,33 +206,27 @@ Definition CCA_EVAL_pkg_ff:
       #val #[decrypt]: 'word × 'word → 'option 'word ] :=
   [package
     #def #[eavesdrop] ('(ml, mr): 'word × 'word): 'word × 'word {
-      S ← get cca_set_location ;;
-      ke ← kgen CCA_EVAL_locs_enc_key ;;
-      km ← kgen CCA_EVAL_locs_mac_key ;;
+      S ← get S_loc ;;
+      ke ← kgen ek_loc ;;
+      km ← kgen km_loc ;;
       let c := enc ke mr in
       let t := mac km c in
-      #put cca_set_location := (setm S (c, t) tt) ;;
+      #put S_loc := setm S (c, t) tt ;;
       ret (c, t)
     } ;
     #def #[decrypt] ('(c, t): 'word × 'word): 'option 'word {
-      S ← get cca_set_location ;;
+      S ← get S_loc ;;
       if ((c, t) \in domm S) then ret None else
-      km ← kgen CCA_EVAL_locs_mac_key ;;
+      km ← kgen km_loc ;;
       if (t != mac km c) then ret None else
-      ke ← kgen CCA_EVAL_locs_enc_key ;;
+      ke ← kgen ek_loc ;;
       ret (Some (dec ke c))
     }
   ].
 
 Definition CCA_EVAL := mkpair CCA_EVAL_pkg_tt CCA_EVAL_pkg_ff.
 
-Definition CCA_EVAL_TAG_locs := fset [:: enc_key_location; cca_set_location].
-
-Lemma CCA_EVAL_TAG_locs_enc_key:
-  enc_key_location \in CCA_EVAL_TAG_locs.
-Proof.
-  auto_in_fset.
-Qed.
+Definition CCA_EVAL_TAG_locs := fset [:: ek_loc; S_loc].
 
 Definition CCA_EVAL_TAG_pkg_tt:
   package CCA_EVAL_TAG_locs
@@ -261,20 +239,20 @@ Definition CCA_EVAL_TAG_pkg_tt:
   [package
     #def #[eavesdrop] ('(ml, mr): 'word × 'word): 'word × 'word {
       #import {sig #[gettag]: 'word → 'word } as gettag ;;
-      S ← get cca_set_location ;;
-      ke ← kgen CCA_EVAL_TAG_locs_enc_key ;;
+      S ← get S_loc ;;
+      ke ← kgen ek_loc ;;
       let c := enc ke ml in
       t ← gettag c ;;
-      #put cca_set_location := (setm S (c, t) tt) ;;
+      #put S_loc := setm S (c, t) tt ;;
       ret (c, t)
     } ;
     #def #[decrypt] ('(c, t): 'word × 'word): 'option 'word {
       #import {sig #[checktag]: 'word × 'word → 'bool } as checktag ;;
-      S ← get cca_set_location ;;
+      S ← get S_loc ;;
       if ((c, t) \in domm S) then ret None else
       r ← checktag (c, t) ;;
       if (~~ r) then ret None else
-      ke ← kgen CCA_EVAL_TAG_locs_enc_key ;;
+      ke ← kgen ek_loc ;;
       ret (Some (dec ke c))
     }
   ].
@@ -290,31 +268,25 @@ Definition CCA_EVAL_TAG_pkg_ff:
   [package
     #def #[eavesdrop] ('(ml, mr): 'word × 'word): 'word × 'word {
       #import {sig #[gettag]: 'word → 'word } as gettag ;;
-      S ← get cca_set_location ;;
-      ke ← kgen CCA_EVAL_TAG_locs_enc_key ;;
+      S ← get S_loc ;;
+      ke ← kgen ek_loc ;;
       let c := enc ke mr in
       t ← gettag c ;;
-      #put cca_set_location := (setm S (c, t) tt) ;;
+      #put S_loc := setm S (c, t) tt ;;
       ret (c, t)
     } ;
     #def #[decrypt] ('(c, t): 'word × 'word): 'option 'word {
       #import {sig #[checktag]: 'word × 'word → 'bool } as checktag ;;
-      S ← get cca_set_location ;;
+      S ← get S_loc ;;
       if ((c, t) \in domm S) then ret None else
       r ← checktag (c, t) ;;
       if (~~ r) then ret None else
-      ke ← kgen CCA_EVAL_TAG_locs_enc_key ;;
+      ke ← kgen ek_loc ;;
       ret (Some (dec ke c))
     }
   ].
 
-Definition CCA_EVAL_HYB_locs := fset [:: mac_key_location; mac_set_location; cca_set_location].
-
-Lemma CCA_EVAL_HYB_locs_mac_key:
-  mac_key_location \in CCA_EVAL_HYB_locs.
-Proof.
-  auto_in_fset.
-Qed.
+Definition CCA_EVAL_HYB_locs := fset [:: km_loc; T_loc; S_loc].
 
 Definition CCA_EVAL_HYB_pkg:
   package CCA_EVAL_HYB_locs
@@ -325,13 +297,13 @@ Definition CCA_EVAL_HYB_pkg:
   [package
     #def #[eavesdrop] ('(ml, mr): 'word × 'word): 'word × 'word {
       #import {sig #[eavesdrop]: 'word × 'word → 'word } as eavesdrop ;;
-      S ← get cca_set_location ;;
+      S ← get S_loc ;;
       c ← eavesdrop (ml, mr) ;;
-      T ← get mac_set_location ;;
-      km ← kgen CCA_EVAL_HYB_locs_mac_key ;;
+      T ← get T_loc ;;
+      km ← kgen km_loc ;;
       let t := mac km c in
-      #put mac_set_location := (setm T (c, t) tt) ;;
-      #put cca_set_location := (setm S (c, t) tt) ;;
+      #put T_loc := setm T (c, t) tt ;;
+      #put S_loc := setm S (c, t) tt ;;
       ret (c, t)
     } ;
     #def #[decrypt] ('(c, t): 'word × 'word): 'option 'word {
@@ -357,7 +329,7 @@ Lemma CCA_EVAL_HYB_equiv_true:
 Proof.
   apply eq_rel_perf_ind with (
     (fun '(h0, h1) => h0 = h1) ⋊
-    couple_lhs cca_set_location mac_set_location
+    couple_lhs S_loc T_loc
       (fun S T => S = T)
   ).
   1: {
@@ -381,7 +353,7 @@ Proof.
     2,4: ssprove_sync=> km;
       ssprove_sync;
       first by move=> ? ? ->.
-    all: apply: (r_rem_couple_lhs cca_set_location mac_set_location) => Hinv.
+    all: apply: (r_rem_couple_lhs S_loc T_loc) => Hinv.
     all: apply: r_put_vs_put.
     all: apply: r_put_vs_put.
     all: ssprove_restore_mem;
@@ -394,7 +366,7 @@ Proof.
     all: rewrite Heq.
     1: by apply: r_ret => ? ? [].
     apply: r_get_remember_lhs => T.
-    apply: (r_rem_couple_lhs cca_set_location mac_set_location) => Hinv.
+    apply: (r_rem_couple_lhs S_loc T_loc) => Hinv.
     rewrite -Hinv Heq /=.
     by apply: r_ret => ? ? [] [].
 Qed.
@@ -404,7 +376,7 @@ Lemma CCA_EVAL_HYB_equiv_false:
 Proof.
   apply eq_rel_perf_ind with (
     (fun '(h0, h1) => h0 = h1) ⋊
-    couple_rhs cca_set_location mac_set_location
+    couple_rhs S_loc T_loc
       (fun S T => S = T)
   ).
   1: {
@@ -428,7 +400,7 @@ Proof.
     2,4: ssprove_sync=> km;
       ssprove_sync;
       first by move=> ? ? ->.
-    all: apply: (r_rem_couple_rhs cca_set_location mac_set_location) => Hinv.
+    all: apply: (r_rem_couple_rhs S_loc T_loc) => Hinv.
     all: apply: r_put_vs_put.
     all: apply: r_put_vs_put.
     all: ssprove_restore_mem;
@@ -441,7 +413,7 @@ Proof.
     all: rewrite Heq.
     1: by apply: r_ret => ? ? [].
     apply: r_get_remember_rhs => T.
-    apply: (r_rem_couple_rhs cca_set_location mac_set_location) => Hinv.
+    apply: (r_rem_couple_rhs S_loc T_loc) => Hinv.
     rewrite -Hinv Heq /=.
     by apply: r_ret => ? ? [] [].
 Qed.
